Commit before changing well_behaved ffi

pancake/proofs/time_to_panProofScript.sml
@@ -1428,6 +1428,206 @@ Proof
 QED
 
 
+Theorem comp_condition_true_correct:
+  ∀s cnd (t:('a,'b) panSem$state) clks clkvals.
+    evalCond s cnd ∧
+    EVERY (λe. case (evalExpr s e) of
+               | SOME n => n < dimword (:α)
+               | _ => F) (destCond cnd) ∧
+    EVERY (λck. MEM ck clks) (condClks cnd) ∧
+    FLOOKUP t.locals «clks» = SOME (Struct clkvals) ∧
+    equiv_val s.clocks clks clkvals ⇒
+    eval t (compCondition clks «clks» cnd) = SOME (ValWord 1w)
+Proof
+  rw [] >>
+  cases_on ‘cnd’ >>
+  fs [evalCond_def, timeLangTheory.condClks_def,
+      timeLangTheory.destCond_def, timeLangTheory.clksOfExprs_def] >>
+  every_case_tac >> fs [] >>
+  qpat_x_assum ‘_ < dimword (:α)’ mp_tac >>
+  qpat_x_assum ‘_ < dimword (:α)’ assume_tac >>
+  strip_tac >>
+  dxrule LESS_MOD >>
+  dxrule LESS_MOD >>
+  strip_tac >> strip_tac
+  >- (
+   dxrule comp_exp_correct >>
+   disch_then
+   (qspecl_then [‘clks’, ‘t’, ‘clkvals’] mp_tac) >>
+   impl_tac
+   >- (
+     fs [] >>
+     drule exprClks_accumulates >>
+     fs []) >>
+   strip_tac >>
+   dxrule comp_exp_correct >>
+   disch_then
+   (qspecl_then [‘clks’, ‘t’, ‘clkvals’] mp_tac) >>
+   impl_tac
+   >- (
+    fs [EVERY_MEM] >>
+    rw [] >>
+    fs [] >>
+    drule exprClks_sublist_accum >>
+    fs []) >>
+   strip_tac >>
+   fs [compCondition_def] >>
+   fs [eval_def, OPT_MMAP_def] >>
+   gs [] >>
+   fs [asmTheory.word_cmp_def] >>
+   gs [word_lo_n2w] >>
+   gs [LESS_OR_EQ, wordLangTheory.word_op_def]) >>
+  dxrule comp_exp_correct >>
+  disch_then
+  (qspecl_then [‘clks’, ‘t’, ‘clkvals’] mp_tac) >>
+  impl_tac
+  >- (
+  fs [] >>
+  drule exprClks_accumulates >>
+  fs []) >>
+  strip_tac >>
+  dxrule comp_exp_correct >>
+  disch_then
+  (qspecl_then [‘clks’, ‘t’, ‘clkvals’] mp_tac) >>
+  impl_tac
+  >- (
+  fs [EVERY_MEM] >>
+  rw [] >>
+  fs [] >>
+  drule exprClks_sublist_accum >>
+  fs []) >>
+  strip_tac >>
+  fs [compCondition_def] >>
+  fs [eval_def, OPT_MMAP_def] >>
+  gs [] >>
+  fs [asmTheory.word_cmp_def] >>
+  gs [word_lo_n2w]
+QED
+
+
+Theorem map_comp_conditions_true_correct:
+  ∀cnds s (t:('a,'b) panSem$state) clks clkvals.
+    EVERY (λcnd. evalCond s cnd) cnds ∧
+    EVERY
+    (λcnd.
+      EVERY (λe. case (evalExpr s e) of
+                 | SOME n => n < dimword (:α)
+                 | _ => F) (destCond cnd)) cnds ∧
+    EVERY
+    (λcnd. EVERY (λck. MEM ck clks) (condClks cnd)) cnds ∧
+    FLOOKUP t.locals «clks» = SOME (Struct clkvals) ∧
+    equiv_val s.clocks clks clkvals ⇒
+    MAP (eval t o compCondition clks «clks») cnds =
+    MAP (SOME o (λx. ValWord 1w)) cnds
+Proof
+  Induct
+  >- rw [] >>
+  rpt gen_tac >>
+  strip_tac >>
+  fs [] >>
+  drule comp_condition_true_correct >>
+  fs [] >>
+  disch_then drule_all >>
+  strip_tac >>
+  last_x_assum match_mp_tac >>
+  gs [] >>
+  qexists_tac ‘s’ >>
+  gs []
+QED
+
+
+Theorem comp_conditions_true_correct:
+  ∀cnds s (t:('a,'b) panSem$state) clks clkvals.
+    EVERY (λcnd. evalCond s cnd) cnds ∧
+    EVERY
+    (λcnd.
+      EVERY (λe. case (evalExpr s e) of
+                 | SOME n => n < dimword (:α)
+                 | _ => F) (destCond cnd)) cnds ∧
+    EVERY
+    (λcnd. EVERY (λck. MEM ck clks) (condClks cnd)) cnds ∧
+    FLOOKUP t.locals «clks» = SOME (Struct clkvals) ∧
+    equiv_val s.clocks clks clkvals ⇒
+    eval t (compConditions clks «clks» cnds) = SOME (ValWord 1w)
+Proof
+  rw [] >>
+  drule map_comp_conditions_true_correct >>
+  gs [] >>
+  disch_then drule_all >>
+  strip_tac >>
+  pop_assum mp_tac >>
+  rpt (pop_assum kall_tac) >>
+  MAP_EVERY qid_spec_tac [‘t’,‘clks’,‘cnds’] >>
+  Induct >> rw []
+  >- (
+    fs [compConditions_def] >>
+    fs [eval_def]) >>
+  fs [compConditions_def] >>
+  fs [eval_def, OPT_MMAP_def] >>
+  fs [GSYM MAP_MAP_o] >>
+  fs [GSYM opt_mmap_eq_some] >>
+  ‘MAP (λx. ValWord 1w) cnds =
+   REPLICATE (LENGTH cnds) (ValWord 1w)’ by (
+    once_rewrite_tac [GSYM map_replicate] >>
+    once_rewrite_tac [GSYM map_replicate] >>
+    once_rewrite_tac [GSYM map_replicate] >>
+    rewrite_tac  [MAP_MAP_o] >>
+    rewrite_tac [MAP_EQ_EVERY2] >>
+    fs [LIST_REL_EL_EQN] >>
+    rw [] >> fs [] >>
+    ‘EL n (REPLICATE (LENGTH cnds) (1:num)) = 1’ by (
+      match_mp_tac EL_REPLICATE >>
+      fs []) >>
+    fs []) >>
+  fs [] >>
+  rewrite_tac [ETA_AX] >>
+  gs [] >>
+  fs [wordLangTheory.word_op_def] >>
+  cheat
+QED
+
+
+Theorem pickTerm_output_cons_correct:
+  ∀s out cnds tclks dest wt s' t (clkvals:'a v list) clks
+   ffi_name nffi nbytes bytes tms.
+    EVERY (λcnd. evalCond s cnd) cnds ∧
+    evalTerm s NONE (Tm (Output out) cnds tclks dest wt) s' ∧
+    EVERY
+    (λcnd.
+      EVERY (λe. case (evalExpr s e) of
+                 | SOME n => n < dimword (:α)
+                 | _ => F) (destCond cnd)) cnds ∧
+    EVERY
+    (λcnd. EVERY (λck. MEM ck clks) (condClks cnd)) cnds ∧
+    FLOOKUP t.locals «clks» = SOME (Struct clkvals) ∧
+    equiv_val s.clocks clks clkvals ∧
+    maxClksSize clkvals ∧
+    clock_bound s.clocks clks (dimword (:'a)) ∧
+    time_range wt (dimword (:'a)) ∧
+    valid_clks clks tclks wt ∧
+    toString dest IN FDOM t.code ∧
+     well_behaved_ffi (strlit (toString out)) t nffi nbytes bytes
+                      (w2n (ffiBufferSize:'a word)) (dimword (:α)) ⇒
+    evaluate (compTerms clks «clks» (Tm (Output out) cnds tclks dest wt::tms), t) =
+    (SOME (Return (retVal s clks tclks wt dest)),
+       t with
+       <|locals :=
+         restore_from t FEMPTY [«len2»; «ptr2»; «len1»; «ptr1»;
+                                «waitTimes»; «newClks»; «wakeUpAt»; «waitSet»];
+         memory := write_bytearray 4000w nbytes t.memory t.memaddrs t.be;
+         ffi := nffi_state t nffi out bytes nbytes|>)
+Proof
+  rw [] >>
+  drule_all comp_conditions_true_correct >>
+  strip_tac >>
+  fs [compTerms_def] >>
+  once_rewrite_tac [evaluate_def] >>
+  fs [timeLangTheory.termConditions_def] >>
+  drule_all comp_output_term_correct >>
+  fs []
+QED
+
+
 
 Theorem state_rel_imp_time_seq_ffi:
   ∀cks s t.
@@ -2705,9 +2905,9 @@ QED
 
 
 (* I think we should have two scenerios *)
-(* lets start when systime is equal to wakehup time,
+(* lets start when systime is equal to wakeup time,
     this way we will not have to execute the while loop
- *)
+*)
 
 Theorem output_step:
   !prog os s s' w (t:('a,time_input) panSem$state) st ns.
@@ -2792,8 +2992,391 @@ Proof
   fs [] >>
   pop_assum kall_tac >>
   pop_assum kall_tac >>
-
   cheat
 QED
+
+
+(* we have pickTerm_ind *)
+(* first proceed in the same direction *)
+
+(*
+Theorem pickTerm_output_cons_correct:
+  ∀s out cnds tclks dest wt s' t (clkvals:'a v list) clks
+   ffi_name nffi nbytes bytes tms.
+
+
+    FLOOKUP t.locals «clks» = SOME (Struct clkvals) ∧
+    equiv_val s.clocks clks clkvals ∧
+    maxClksSize clkvals ∧
+    clk_range s.clocks clks (dimword (:'a)) ∧
+    time_range wt (dimword (:'a)) ∧
+    valid_clks clks tclks wt ∧
+    toString dest IN FDOM t.code ∧
+    well_behaved_ffi (strlit (toString out)) t nffi nbytes bytes (dimword (:α)) ⇒
+    evaluate (compTerms clks «clks» (Tm (Output out) cnds tclks dest wt::tms), t) =
+    (SOME (Return (retVal s clks tclks wt dest)),
+       t with
+       <|locals :=
+         restore_from t FEMPTY [«len2»; «ptr2»; «len1»; «ptr1»;
+                                «waitTimes»; «newClks»; «wakeUpAt»; «waitSet»];
+         memory := write_bytearray 4000w nbytes t.memory t.memaddrs t.be;
+         ffi := nffi_state t nffi out bytes nbytes|>)
+*)
+
+
+Definition conds_eval_lt_dimword_def:
+  conds_eval_lt_dimword (:'a) s tms =
+    EVERY (λtm.
+            EVERY (λcnd.
+                    EVERY (λe. case (evalExpr s e) of
+                               | SOME n => n < dimword (:α)
+                               | _ => F) (destCond cnd))
+                  (termConditions tm)
+          ) tms
+End
+
+
+Definition conds_clks_mem_clks_def:
+  conds_clks_mem_clks clks tms =
+    EVERY (λtm.
+            EVERY (λcnd.
+                    EVERY (λck. MEM ck clks) (condClks cnd))
+                  (termConditions tm)
+          ) tms
+End
+
+Definition terms_time_range_def:
+  terms_time_range (:'a) tms =
+    EVERY (λtm.
+            time_range (termWaitTimes tm) (dimword (:'a))
+          ) tms
+End
+
+Definition terms_valid_clocks_def:
+  terms_valid_clocks clks tms  =
+    EVERY (λtm.
+            valid_clks clks (termClks tm) (termWaitTimes tm)
+          ) tms
+End
+
+Definition locs_in_code_def:
+  locs_in_code fm tms =
+    EVERY (λtm.
+            toString (termDest tm) IN FDOM fm
+          ) tms
+End
+
+
+
+Theorem foo:
+  ∀s e tms s'.
+    pickTerm s e tms s' ⇒
+    (∀(t :('a, 'b) panSem$state) clks clkvals.
+       e = NONE ∧
+       conds_eval_lt_dimword (:'a) s tms ∧
+       conds_clks_mem_clks clks tms ∧
+       terms_time_range (:'a) tms ∧
+       terms_valid_clocks clks tms ∧
+       locs_in_code t.code tms ∧
+       FLOOKUP t.locals «clks» = SOME (Struct clkvals) ∧
+       equiv_val s.clocks clks clkvals ∧
+       maxClksSize clkvals ∧
+       clock_bound s.clocks clks (dimword (:'a))  ⇒
+       ∃out cnds tclks dest wt.
+         MEM (Tm (Output out) cnds tclks dest wt) tms ∧
+         evaluate (compTerms clks «clks» tms, t) =
+         (SOME (Return (retVal s clks tclks wt dest)),
+          t with
+            <|locals :=
+              restore_from t FEMPTY [«len2»; «ptr2»; «len1»; «ptr1»;
+                                     «waitTimes»; «newClks»; «wakeUpAt»; «waitSet»];
+              memory := write_bytearray 4000w nbytes t.memory t.memaddrs t.be;
+              ffi := nffi_state t nffi out bytes nbytes|>))
+Proof
+  ho_match_mp_tac pickTerm_ind >>
+  rw []
+  >- (
+    MAP_EVERY qexists_tac
+              [‘out_signal’, ‘cnds’, ‘clks’, ‘dest’, ‘diffs'’] >>
+    fs [] >>
+    match_mp_tac pickTerm_output_cons_correct >>
+    qexists_tac ‘s'’ >>
+    qexists_tac ‘clkvals’ >>
+    qexists_tac ‘ffi_name’ >>
+    gs [] >>
+    conj_tac
+    >- gs [conds_eval_lt_dimword_def, timeLangTheory.termConditions_def] >>
+    conj_tac
+    >- gs [conds_clks_mem_clks_def, timeLangTheory.termConditions_def] >>
+    conj_tac
+    >- gs [terms_time_range_def, timeLangTheory.termWaitTimes_def] >>
+    conj_tac
+    >- gs [terms_valid_clocks_def, timeLangTheory.termClks_def,
+           timeLangTheory.termWaitTimes_def] >>
+    conj_tac
+    >- gs [locs_in_code_def, timeLangTheory.termDest_def] >>
+    cheat)
+
+
+
+
+
+
+
+
+
+
+
+  )
+  >- (
+    last_x_assum (qspecl_then [‘clks'’, ‘t’] assume_tac) >>
+    fs [] >>
+    MAP_EVERY qexists_tac
+              [‘out’, ‘cnds'’, ‘tclks’, ‘dest'’, ‘wt’] >>
+    fs [] >>
+    cheat) >>
+
+
+
+
+
+
+    )
+
+
+  )
+  drule_all comp_conditions_true_correct >>
+  strip_tac >>
+  fs [compTerms_def] >>
+  once_rewrite_tac [evaluate_def] >>
+  fs [timeLangTheory.termConditions_def] >>
+  drule_all comp_output_term_correct >>
+  fs []
+QED
+
+
+
+
+
+
+
+Theorem foo:
+  ∀tms s s' clks.
+    pickTerm s NONE tms s' ⇒
+    ∃out cnds tclks dest wt.
+      MEM (Tm (Output out) cnds tclks dest wt) tms ∧
+      evaluate (compTerms clks «clks» tms, t) =
+      (SOME (Return (retVal s clks tclks wt dest)), ARB t)
+Proof
+  Induct >>
+  rw []
+  >- (
+  fs [pickTerm_def]
+
+
+  )
+  drule_all comp_conditions_true_correct >>
+  strip_tac >>
+  fs [compTerms_def] >>
+  once_rewrite_tac [evaluate_def] >>
+  fs [timeLangTheory.termConditions_def] >>
+  drule_all comp_output_term_correct >>
+  fs []
+QED
+
+
+
+
+
+
+
+
+
+
+Theorem comp_condition_false_correct:
+  ∀s cnd (t:('a,'b) panSem$state) clks clkvals.
+    ~(evalCond s cnd) ∧
+    EVERY (λe. case (evalExpr s e) of
+               | SOME n => n < dimword (:α)
+               | _ => F) (destCond cnd) ∧
+    EVERY (λck. MEM ck clks) (condClks cnd) ∧
+    FLOOKUP t.locals «clks» = SOME (Struct clkvals) ∧
+    equiv_val s.clocks clks clkvals ⇒
+    eval t (compCondition clks «clks» cnd) = SOME (ValWord 0w)
+Proof
+  rw [] >>
+  cases_on ‘cnd’ >>
+  fs [evalCond_def, timeLangTheory.condClks_def,
+      timeLangTheory.destCond_def, timeLangTheory.clksOfExprs_def] >>
+  every_case_tac >> fs []
+  >- (
+   dxrule comp_exp_correct >>
+   disch_then
+   (qspecl_then [‘clks’, ‘t’, ‘clkvals’] mp_tac) >>
+   impl_tac
+   >- (
+     fs [] >>
+     drule exprClks_accumulates >>
+     fs []) >>
+   strip_tac >>
+   dxrule comp_exp_correct >>
+   disch_then
+   (qspecl_then [‘clks’, ‘t’, ‘clkvals’] mp_tac) >>
+   impl_tac
+   >- (
+    fs [EVERY_MEM] >>
+    rw [] >>
+    fs [] >>
+    drule exprClks_sublist_accum >>
+    fs []) >>
+   strip_tac >>
+   fs [compCondition_def] >>
+   fs [eval_def, OPT_MMAP_def] >>
+   gs [] >>
+   fs [asmTheory.word_cmp_def] >>
+   gs [word_lo_n2w] >>
+   fs [wordLangTheory.word_op_def]) >>
+  dxrule comp_exp_correct >>
+  disch_then
+  (qspecl_then [‘clks’, ‘t’, ‘clkvals’] mp_tac) >>
+  impl_tac
+  >- (
+    fs [] >>
+    drule exprClks_accumulates >>
+    fs []) >>
+  strip_tac >>
+  dxrule comp_exp_correct >>
+  disch_then
+  (qspecl_then [‘clks’, ‘t’, ‘clkvals’] mp_tac) >>
+  impl_tac
+  >- (
+    fs [EVERY_MEM] >>
+    rw [] >>
+    fs [] >>
+    drule exprClks_sublist_accum >>
+    fs []) >>
+  strip_tac >>
+  fs [compCondition_def] >>
+  fs [eval_def, OPT_MMAP_def] >>
+  gs [] >>
+  fs [asmTheory.word_cmp_def] >>
+  gs [word_lo_n2w]
+QED
+
+
+(* when each condition is true and input signals match with the first term *)
+Theorem pickTerm_input_cons_correct:
+  ∀s n cnds tclks dest wt s' t (clkvals:'a v list) clks tms.
+    EVERY (λcnd. evalCond s cnd) cnds ∧
+    evalTerm s (SOME n) (Tm (Input n) cnds tclks dest wt) s' ∧
+    EVERY
+    (λcnd.
+      EVERY (λe. case (evalExpr s e) of
+                 | SOME n => n < dimword (:α)
+                 | _ => F) (destCond cnd)) cnds ∧
+    EVERY
+    (λcnd. EVERY (λck. MEM ck clks) (condClks cnd)) cnds ∧
+    FLOOKUP t.locals «clks» = SOME (Struct clkvals) ∧
+    equiv_val s.clocks clks clkvals ∧
+    maxClksSize clkvals ∧
+    clk_range s.clocks clks (dimword (:'a)) ∧
+    time_range wt (dimword (:'a)) ∧
+    valid_clks clks tclks wt ∧
+    toString dest IN FDOM t.code ⇒
+    evaluate (compTerms clks «clks» (Tm (Input n) cnds tclks dest wt::tms), t) =
+    (SOME (Return (retVal s clks tclks wt dest)),
+     t with locals :=
+     restore_from t FEMPTY [«waitTimes»; «newClks»; «wakeUpAt»; «waitSet»])
+Proof
+  rw [] >>
+  drule_all comp_conditions_true_correct >>
+  strip_tac >>
+  fs [compTerms_def] >>
+  once_rewrite_tac [evaluate_def] >>
+  fs [timeLangTheory.termConditions_def] >>
+  drule_all comp_input_term_correct >>
+  fs []
+QED
+
+(* when each condition is true and output signals match with the first term *)
+Theorem pickTerm_output_cons_correct:
+  ∀s out cnds tclks dest wt s' t (clkvals:'a v list) clks
+   ffi_name nffi nbytes bytes tms.
+    EVERY (λcnd. evalCond s cnd) cnds ∧
+    evalTerm s NONE (Tm (Output out) cnds tclks dest wt) s' ∧
+    EVERY
+    (λcnd.
+      EVERY (λe. case (evalExpr s e) of
+                 | SOME n => n < dimword (:α)
+                 | _ => F) (destCond cnd)) cnds ∧
+    EVERY
+    (λcnd. EVERY (λck. MEM ck clks) (condClks cnd)) cnds ∧
+    FLOOKUP t.locals «clks» = SOME (Struct clkvals) ∧
+    equiv_val s.clocks clks clkvals ∧
+    maxClksSize clkvals ∧
+    clk_range s.clocks clks (dimword (:'a)) ∧
+    time_range wt (dimword (:'a)) ∧
+    valid_clks clks tclks wt ∧
+    toString dest IN FDOM t.code ∧
+    well_behaved_ffi (strlit (toString out)) t nffi nbytes bytes (dimword (:α)) ⇒
+    evaluate (compTerms clks «clks» (Tm (Output out) cnds tclks dest wt::tms), t) =
+    (SOME (Return (retVal s clks tclks wt dest)),
+       t with
+       <|locals :=
+         restore_from t FEMPTY [«len2»; «ptr2»; «len1»; «ptr1»;
+                                «waitTimes»; «newClks»; «wakeUpAt»; «waitSet»];
+         memory := write_bytearray 4000w nbytes t.memory t.memaddrs t.be;
+         ffi := nffi_state t nffi out bytes nbytes|>)
+Proof
+  rw [] >>
+  drule_all comp_conditions_true_correct >>
+  strip_tac >>
+  fs [compTerms_def] >>
+  once_rewrite_tac [evaluate_def] >>
+  fs [timeLangTheory.termConditions_def] >>
+  drule_all comp_output_term_correct >>
+  fs []
+QED
+
+
+Theorem pickTerm_true_imp_evalTerm:
+  ∀s io tms s'.
+    pickTerm s io tms s' ⇒
+    ∃tm. MEM tm tms ∧ EVERY (λcnd. evalCond s cnd) (termConditions tm) ∧
+         case tm of
+         | Tm (Input n) cnds tclks dest wt =>
+             evalTerm s (SOME n) (Tm (Input n) cnds tclks dest wt) s'
+         | Tm (Output out) cnds tclks dest wt =>
+             evalTerm s NONE (Tm (Output out) cnds tclks dest wt) s'
+Proof
+  ho_match_mp_tac pickTerm_ind >>
+  rw [] >> fs []
+  >- (
+  qexists_tac ‘Tm (Input in_signal) cnds clks dest diffs'’ >>
+  fs [timeLangTheory.termConditions_def])
+  >- (
+  qexists_tac ‘Tm (Output out_signal) cnds clks dest diffs'’ >>
+  fs [timeLangTheory.termConditions_def]) >>
+  qexists_tac ‘tm’ >> fs []
+QED
+
+
+(* when any condition is false, but there is a matching term, then we can append the
+   list with the false term  *)
+Theorem pickTerm_last_cases:
+  ∀s event io cnds tclks dest wt s' t (clkvals:'a v list) clks tms.
+    ~(EVERY (λcnd. evalCond s cnd) cnds) ∧
+    pickTerm s event tms s' ⇒
+    evaluate (compTerms clks «clks» (Tm io cnds tclks dest wt::tms), t) =
+    evaluate (compTerms clks «clks» tm, t)
+Proof
+  rw [] >>
+  drule pickTerm_true_imp_evalTerm >>
+  strip_tac >>
+  fs [] >>
+  (* we can go on, but first I should see what kind of lemmas are needed *)
+  cheat
+QED
+
 
 val _ = export_theory();
